rr_frontend/output/minivec_patched/generated_code_minivec.v
@@ -1,0 +1,1574 @@
+From caesium Require Import lang notation.
+From refinedrust Require Import typing.
+
+Section RawVec_sls.
+  Context `{!typeGS Σ}.
+
+  Definition RawVec_sls (T_st : syn_type) : struct_layout_spec := mk_sls "RawVec" [
+    ("ptr", PtrSynType);
+    ("cap", IntSynType USize);
+    ("_marker", UnitSynType)].
+End RawVec_sls.
+
+Section Vec_sls.
+  Context `{!typeGS Σ}.
+
+  Definition Vec_sls (T_st : syn_type) : struct_layout_spec := mk_sls "Vec" [
+    ("buf", (syn_type_of_sls ((RawVec_sls (T_st)))));
+    ("len", IntSynType USize)].
+End Vec_sls.
+
+Section std_option_Option_els.
+  Context `{!typeGS Σ}.
+
+  Definition std_option_Option_None_sls  : struct_layout_spec := mk_sls "std_option_Option_None" [].
+
+  Definition std_option_Option_Some_sls T_st : struct_layout_spec := mk_sls "std_option_Option_Some" [
+    ("0", T_st)].
+
+  Program Definition std_option_Option_els (T_st : syn_type): enum_layout_spec := mk_els "std_option_Option" ISize [
+    ("None", std_option_Option_None_sls  : syn_type);
+    ("Some", std_option_Option_Some_sls T_st : syn_type)] [("None", 0); ("Some", 1)] _ _ _ _.
+  Next Obligation. repeat first [econstructor | set_solver]. Qed.
+  Next Obligation. done. Qed.
+  Next Obligation. repeat first [econstructor | set_solver]. Qed.
+  Next Obligation. repeat first [econstructor | solve_goal]. Qed.
+Global Typeclasses Opaque std_option_Option_els.
+End std_option_Option_els.
+
+Section code.
+Context `{!typeGS Σ}.
+Open Scope printing_sugar.
+
+Definition RawVecTasstd_ops_Drop_drop_def (std_mem_size_of_T_loc : loc) (free_array_T_loc : loc) (T_st : syn_type) : function := {|
+ f_args := [
+  ("self", void* : layout)
+ ];
+ f_local_vars := [
+  ("__0", (layout_of unit_sl) : layout);
+  ("elem_size", (it_layout USize) : layout);
+  ("__3", (it_layout U8) : layout);
+  ("__4", (it_layout U8) : layout);
+  ("__5", (it_layout USize) : layout);
+  ("__6", (it_layout U8) : layout);
+  ("__7", (it_layout USize) : layout);
+  ("__8", (layout_of unit_sl) : layout);
+  ("__9", (it_layout USize) : layout);
+  ("__10", void* : layout);
+  ("__11", void* : layout)
+ ];
+ f_code :=
+  <[
+  "_bb7" :=
+   "__0" <-{ StructOp unit_sl [] } zst_val;
+   Goto "_bb8"
+  ]>%E $
+  <[
+  "_bb4" :=
+   if{ BoolOp }: use{ BoolOp } ("__3") then
+    Goto "_bb5"
+   else
+    Goto "_bb7"
+  ]>%E $
+  <[
+  "_bb1" :=
+   "__5" <-{ IntOp USize } use{ IntOp USize } ((!{ PtrOp } ( "self" )) at{ ((RawVec_sls (T_st))) } "cap");
+   "__4" <-{ BoolOp } (use{ IntOp USize } ("__5")) != { IntOp USize , IntOp USize , U8 } (I2v (0) U64);
+   if{ BoolOp }: use{ BoolOp } ("__4") then
+    Goto "_bb3"
+   else
+    Goto "_bb2"
+  ]>%E $
+  <[
+  "_bb0" :=
+   annot: CopyLftNameAnnot "plft4" "ulft__";
+   "elem_size" <-{ IntOp USize } CallE std_mem_size_of_T_loc [] [@{expr} ];
+   Goto "_bb1"
+  ]>%E $
+  <[
+  "_bb8" :=
+   (*annot: StratifyContextAnnot;*)
+   return (use{ StructOp unit_sl [] } ("__0"))
+  ]>%E $
+  <[
+  "_bb6" :=
+   "__0" <-{ StructOp unit_sl [] } zst_val;
+   Goto "_bb8"
+  ]>%E $
+  <[
+  "_bb3" :=
+   "__7" <-{ IntOp USize } use{ IntOp USize } ("elem_size");
+   "__6" <-{ BoolOp } (use{ IntOp USize } ("__7")) != { IntOp USize , IntOp USize , U8 } (I2v (0) U64);
+   "__3" <-{ BoolOp } use{ BoolOp } ("__6");
+   Goto "_bb4"
+  ]>%E $
+  <[
+  "_bb5" :=
+   "__9" <-{ IntOp USize } use{ IntOp USize } ((!{ PtrOp } ( "self" )) at{ ((RawVec_sls (T_st))) } "cap");
+   "__11" <-{ PtrOp } use{ PtrOp } ((!{ PtrOp } ( "self" )) at{ ((RawVec_sls (T_st))) } "ptr");
+   "__10" <-{ PtrOp } use{ PtrOp } ("__11");
+   "__8" <-{ StructOp unit_sl [] } CallE free_array_T_loc [] [@{expr} use{ IntOp USize } ("__9"); use{ PtrOp } ("__10")];
+   Goto "_bb6"
+  ]>%E $
+  <[
+  "_bb2" :=
+   "__3" <-{ BoolOp } val_of_bool false;
+   Goto "_bb4"
+  ]>%E $
+  ∅;
+ f_init := "_bb0";
+|}.
+
+Definition Vec_T_insert_def (std_ptr_write_T_loc : loc) (ptr_add_T_loc : loc) (Vec_T_cap_T_loc : loc) (Vec_T_ptr_T_loc : loc) (RawVec_T_grow_T_loc : loc) (std_ptr_copy_T_loc : loc) (T_st : syn_type) : function := {|
+ f_args := [
+  ("self", void* : layout);
+  ("index", (it_layout USize) : layout);
+  ("elem", (use_layout_alg' T_st) : layout)
+ ];
+ f_local_vars := [
+  ("__0", (layout_of unit_sl) : layout);
+  ("__4", (layout_of unit_sl) : layout);
+  ("__5", (it_layout U8) : layout);
+  ("__6", (it_layout U8) : layout);
+  ("__7", (it_layout USize) : layout);
+  ("__8", (it_layout USize) : layout);
+  ("__9", (layout_of unit_sl) : layout);
+  ("__10", (layout_of unit_sl) : layout);
+  ("__11", (it_layout U8) : layout);
+  ("__12", (it_layout USize) : layout);
+  ("__13", void* : layout);
+  ("__14", (it_layout USize) : layout);
+  ("__15", (layout_of unit_sl) : layout);
+  ("__16", void* : layout);
+  ("__17", (layout_of unit_sl) : layout);
+  ("__18", void* : layout);
+  ("__19", void* : layout);
+  ("__20", void* : layout);
+  ("__21", void* : layout);
+  ("__22", (it_layout USize) : layout);
+  ("__23", void* : layout);
+  ("__24", void* : layout);
+  ("__25", void* : layout);
+  ("__26", (it_layout USize) : layout);
+  ("__27", (it_layout USize) : layout);
+  ("__28", (it_layout USize) : layout);
+  ("__29", (it_layout USize) : layout);
+  ("__30", (it_layout USize) : layout);
+  ("__31", (it_layout USize) : layout);
+  ("__32", (it_layout USize) : layout);
+  ("__33", (layout_of unit_sl) : layout);
+  ("__34", void* : layout);
+  ("__35", void* : layout);
+  ("__36", void* : layout);
+  ("__37", (it_layout USize) : layout);
+  ("__38", (use_layout_alg' T_st) : layout);
+  ("__39", (it_layout USize) : layout)
+ ];
+ f_code :=
+  <[
+  "_bb13" :=
+   "__29" <-{ IntOp USize } use{ IntOp USize } ("__32");
+   "__17" <-{ StructOp unit_sl [] } CallE std_ptr_copy_T_loc [] [@{expr} use{ PtrOp } ("__18"); use{ PtrOp } ("__23"); use{ IntOp USize } ("__29")];
+   Goto "_bb14"
+  ]>%E $
+  <[
+  "_bb19" :=
+   (*annot: StratifyContextAnnot;*)
+   return (use{ StructOp unit_sl [] } ("__0"))
+  ]>%E $
+  <[
+  "_bb1" :=
+   StuckS
+  ]>%E $
+  <[
+  "_bb17" :=
+   "__39" <-{ IntOp USize } (use{ IntOp USize } ((!{ PtrOp } ( "self" )) at{ ((Vec_sls (T_st))) } "len")) +c{ IntOp USize , IntOp USize } (I2v (1) U64);
+   assert{ BoolOp }: (val_of_bool false) = { BoolOp , BoolOp , U8 } (val_of_bool false);
+   Goto "_bb18"
+  ]>%E $
+  <[
+  "_bb4" :=
+   annot: StartLftAnnot "llft7" ["plft11"];
+   "__16" <-{ PtrOp } AnnotExpr 0 (GetLftNamesAnnot (LftNameTreeRef "plft13" (LftNameTreeLeaf))) (&ref{ Mut, Some (RSTLitType ["RawVec_inv_t"] [RSTTyVar "T"]), "llft7" } ((!{ PtrOp } ( "self" )) at{ ((Vec_sls (T_st))) } "buf"));
+   annot: CopyLftNameAnnot "plft18" "plft13";
+   "__15" <-{ StructOp unit_sl [] } CallE RawVec_T_grow_T_loc ["plft18"] [@{expr} use{ PtrOp } ("__16")];
+   annot: EndLftAnnot "llft7";
+   Goto "_bb5"
+  ]>%E $
+  <[
+  "_bb8" :=
+   annot: EndLftAnnot "llft8";
+   "__22" <-{ IntOp USize } use{ IntOp USize } ("index");
+   "__19" <-{ PtrOp } CallE ptr_add_T_loc [] [@{expr} use{ PtrOp } ("__20"); use{ IntOp USize } ("__22")];
+   Goto "_bb9"
+  ]>%E $
+  <[
+  "_bb15" :=
+   annot: EndLftAnnot "llft10";
+   "__37" <-{ IntOp USize } use{ IntOp USize } ("index");
+   "__34" <-{ PtrOp } CallE ptr_add_T_loc [] [@{expr} use{ PtrOp } ("__35"); use{ IntOp USize } ("__37")];
+   Goto "_bb16"
+  ]>%E $
+  <[
+  "_bb12" :=
+   "__30" <-{ IntOp USize } use{ IntOp USize } ((!{ PtrOp } ( "self" )) at{ ((Vec_sls (T_st))) } "len");
+   "__31" <-{ IntOp USize } use{ IntOp USize } ("index");
+   "__32" <-{ IntOp USize } (use{ IntOp USize } ("__30")) -c{ IntOp USize , IntOp USize } (use{ IntOp USize } ("__31"));
+   assert{ BoolOp }: (val_of_bool false) = { BoolOp , BoolOp , U8 } (val_of_bool false);
+   Goto "_bb13"
+  ]>%E $
+  <[
+  "_bb2" :=
+   "__4" <-{ StructOp unit_sl [] } zst_val;
+   annot: StartLftAnnot "llft6" ["plft11"];
+   "__13" <-{ PtrOp } AnnotExpr 0 (GetLftNamesAnnot (LftNameTreeRef "plft12" (LftNameTreeLeaf))) (&ref{ Shr, None, "llft6" } (!{ PtrOp } ( "self" )));
+   annot: CopyLftNameAnnot "plft17" "plft12";
+   "__12" <-{ IntOp USize } CallE Vec_T_cap_T_loc ["plft17"] [@{expr} use{ PtrOp } ("__13")];
+   annot: EndLftAnnot "llft6";
+   Goto "_bb3"
+  ]>%E $
+  <[
+  "_bb16" :=
+   "__38" <-{ (use_op_alg' T_st) } use{ (use_op_alg' T_st) } ("elem");
+   "__33" <-{ StructOp unit_sl [] } CallE std_ptr_write_T_loc [] [@{expr} use{ PtrOp } ("__34"); use{ (use_op_alg' T_st) } ("__38")];
+   Goto "_bb17"
+  ]>%E $
+  <[
+  "_bb6" :=
+   "__10" <-{ StructOp unit_sl [] } zst_val;
+   Goto "_bb7"
+  ]>%E $
+  <[
+  "_bb11" :=
+   "__26" <-{ IntOp USize } use{ IntOp USize } ("__28");
+   "__23" <-{ PtrOp } CallE ptr_add_T_loc [] [@{expr} use{ PtrOp } ("__24"); use{ IntOp USize } ("__26")];
+   Goto "_bb12"
+  ]>%E $
+  <[
+  "_bb0" :=
+   annot: CopyLftNameAnnot "plft11" "ulft__";
+   "__7" <-{ IntOp USize } use{ IntOp USize } ("index");
+   "__8" <-{ IntOp USize } use{ IntOp USize } ((!{ PtrOp } ( "self" )) at{ ((Vec_sls (T_st))) } "len");
+   "__6" <-{ BoolOp } (use{ IntOp USize } ("__7")) ≤{ IntOp USize , IntOp USize , U8 } (use{ IntOp USize } ("__8"));
+   "__5" <-{ BoolOp } UnOp (NotBoolOp) (BoolOp) (use{ BoolOp } ("__6"));
+   if{ BoolOp }: use{ BoolOp } ("__5") then
+    Goto "_bb1"
+   else
+    Goto "_bb2"
+  ]>%E $
+  <[
+  "_bb5" :=
+   annot: EndLftAnnot "llft7";
+   "__10" <-{ StructOp unit_sl [] } zst_val;
+   Goto "_bb7"
+  ]>%E $
+  <[
+  "_bb3" :=
+   annot: EndLftAnnot "llft6";
+   "__14" <-{ IntOp USize } use{ IntOp USize } ((!{ PtrOp } ( "self" )) at{ ((Vec_sls (T_st))) } "len");
+   "__11" <-{ BoolOp } (use{ IntOp USize } ("__12")) = { IntOp USize , IntOp USize , U8 } (use{ IntOp USize } ("__14"));
+   if{ BoolOp }: use{ BoolOp } ("__11") then
+    Goto "_bb4"
+   else
+    Goto "_bb6"
+  ]>%E $
+  <[
+  "_bb7" :=
+   annot: StartLftAnnot "llft8" ["plft11"];
+   "__21" <-{ PtrOp } AnnotExpr 0 (GetLftNamesAnnot (LftNameTreeRef "plft14" (LftNameTreeLeaf))) (&ref{ Shr, None, "llft8" } (!{ PtrOp } ( "self" )));
+   annot: CopyLftNameAnnot "plft19" "plft14";
+   "__20" <-{ PtrOp } CallE Vec_T_ptr_T_loc ["plft19"] [@{expr} use{ PtrOp } ("__21")];
+   annot: EndLftAnnot "llft8";
+   Goto "_bb8"
+  ]>%E $
+  <[
+  "_bb9" :=
+   "__18" <-{ PtrOp } use{ PtrOp } ("__19");
+   annot: StartLftAnnot "llft9" ["plft11"];
+   "__25" <-{ PtrOp } AnnotExpr 0 (GetLftNamesAnnot (LftNameTreeRef "plft15" (LftNameTreeLeaf))) (&ref{ Shr, None, "llft9" } (!{ PtrOp } ( "self" )));
+   annot: CopyLftNameAnnot "plft20" "plft15";
+   "__24" <-{ PtrOp } CallE Vec_T_ptr_T_loc ["plft20"] [@{expr} use{ PtrOp } ("__25")];
+   annot: EndLftAnnot "llft9";
+   Goto "_bb10"
+  ]>%E $
+  <[
+  "_bb14" :=
+   annot: StartLftAnnot "llft10" ["plft11"];
+   "__36" <-{ PtrOp } AnnotExpr 0 (GetLftNamesAnnot (LftNameTreeRef "plft16" (LftNameTreeLeaf))) (&ref{ Shr, None, "llft10" } (!{ PtrOp } ( "self" )));
+   annot: CopyLftNameAnnot "plft21" "plft16";
+   "__35" <-{ PtrOp } CallE Vec_T_ptr_T_loc ["plft21"] [@{expr} use{ PtrOp } ("__36")];
+   annot: EndLftAnnot "llft10";
+   Goto "_bb15"
+  ]>%E $
+  <[
+  "_bb10" :=
+   annot: EndLftAnnot "llft9";
+   "__27" <-{ IntOp USize } use{ IntOp USize } ("index");
+   "__28" <-{ IntOp USize } (use{ IntOp USize } ("__27")) +c{ IntOp USize , IntOp USize } (I2v (1) U64);
+   assert{ BoolOp }: (val_of_bool false) = { BoolOp , BoolOp , U8 } (val_of_bool false);
+   Goto "_bb11"
+  ]>%E $
+  <[
+  "_bb18" :=
+   (!{ PtrOp } ( "self" )) at{ ((Vec_sls (T_st))) } "len" <-{ IntOp USize } use{ IntOp USize } ("__39");
+   "__0" <-{ StructOp unit_sl [] } zst_val;
+   (*expr: AnnotExpr 0 DropAnnot ("elem");*)
+   Goto "_bb19"
+  ]>%E $
+  ∅;
+ f_init := "_bb0";
+|}.
+
+Definition main_def : function := {|
+ f_args := [
+ ];
+ f_local_vars := [
+  ("__0", (layout_of unit_sl) : layout)
+ ];
+ f_code :=
+  <[
+  "_bb0" :=
+   "__0" <-{ StructOp unit_sl [] } zst_val;
+   (*annot: StratifyContextAnnot;*)
+   return (use{ StructOp unit_sl [] } ("__0"))
+  ]>%E $
+  ∅;
+ f_init := "_bb0";
+|}.
+
+Definition RawVec_T_with_capacity_def (std_mem_size_of_T_loc : loc) (ptr_dangling_T_loc : loc) (check_array_layoutable_T_loc : loc) (alloc_array_T_loc : loc) (T_st : syn_type) : function := {|
+ f_args := [
+  ("capacity", (it_layout USize) : layout)
+ ];
+ f_local_vars := [
+  ("__0", (use_layout_alg' (syn_type_of_sls ((RawVec_sls (T_st))))) : layout);
+  ("__2", (it_layout U8) : layout);
+  ("__3", (it_layout U8) : layout);
+  ("__4", (it_layout USize) : layout);
+  ("__5", (it_layout U8) : layout);
+  ("__6", (it_layout USize) : layout);
+  ("__7", void* : layout);
+  ("__8", void* : layout);
+  ("__9", (it_layout USize) : layout);
+  ("__10", (layout_of unit_sl) : layout);
+  ("__11", (layout_of unit_sl) : layout);
+  ("__12", (it_layout U8) : layout);
+  ("__13", (it_layout U8) : layout);
+  ("__14", (it_layout USize) : layout);
+  ("__15", (layout_of unit_sl) : layout);
+  ("ptr", void* : layout);
+  ("__17", (it_layout USize) : layout);
+  ("__18", void* : layout);
+  ("__19", void* : layout);
+  ("__20", (it_layout USize) : layout);
+  ("__21", (layout_of unit_sl) : layout)
+ ];
+ f_code :=
+  <[
+  "_bb11" :=
+   "__19" <-{ PtrOp } use{ PtrOp } ("ptr");
+   "__18" <-{ PtrOp } use{ PtrOp } ("__19");
+   "__20" <-{ IntOp USize } use{ IntOp USize } ("capacity");
+   "__21" <-{ StructOp unit_sl [] } zst_val;
+   "__0" <-{ (use_op_alg' (syn_type_of_sls ((RawVec_sls (T_st))))) } StructInit ((RawVec_sls (T_st))) [("ptr", use{ PtrOp } ("__18") : expr); ("cap", use{ IntOp USize } ("__20") : expr); ("_marker", use{ StructOp unit_sl [] } ("__21") : expr)];
+   Goto "_bb12"
+  ]>%E $
+  <[
+  "_bb2" :=
+   "__6" <-{ IntOp USize } use{ IntOp USize } ("capacity");
+   "__5" <-{ BoolOp } (use{ IntOp USize } ("__6")) = { IntOp USize , IntOp USize , U8 } (I2v (0) U64);
+   "__2" <-{ BoolOp } use{ BoolOp } ("__5");
+   Goto "_bb3"
+  ]>%E $
+  <[
+  "_bb9" :=
+   StuckS
+  ]>%E $
+  <[
+  "_bb8" :=
+   "__12" <-{ BoolOp } UnOp (NotBoolOp) (BoolOp) (use{ BoolOp } ("__13"));
+   if{ BoolOp }: use{ BoolOp } ("__12") then
+    Goto "_bb9"
+   else
+    Goto "_bb10"
+  ]>%E $
+  <[
+  "_bb6" :=
+   "__7" <-{ PtrOp } use{ PtrOp } ("__8");
+   "__9" <-{ IntOp USize } use{ IntOp USize } ("capacity");
+   "__10" <-{ StructOp unit_sl [] } zst_val;
+   "__0" <-{ (use_op_alg' (syn_type_of_sls ((RawVec_sls (T_st))))) } StructInit ((RawVec_sls (T_st))) [("ptr", use{ PtrOp } ("__7") : expr); ("cap", use{ IntOp USize } ("__9") : expr); ("_marker", use{ StructOp unit_sl [] } ("__10") : expr)];
+   Goto "_bb12"
+  ]>%E $
+  <[
+  "_bb12" :=
+   (*annot: StratifyContextAnnot;*)
+   return (use{ (use_op_alg' (syn_type_of_sls ((RawVec_sls (T_st))))) } ("__0"))
+  ]>%E $
+  <[
+  "_bb10" :=
+   "__11" <-{ StructOp unit_sl [] } zst_val;
+   "__17" <-{ IntOp USize } use{ IntOp USize } ("capacity");
+   "ptr" <-{ PtrOp } CallE alloc_array_T_loc [] [@{expr} use{ IntOp USize } ("__17")];
+   Goto "_bb11"
+  ]>%E $
+  <[
+  "_bb7" :=
+   "__14" <-{ IntOp USize } use{ IntOp USize } ("capacity");
+   "__13" <-{ BoolOp } CallE check_array_layoutable_T_loc [] [@{expr} use{ IntOp USize } ("__14")];
+   Goto "_bb8"
+  ]>%E $
+  <[
+  "_bb5" :=
+   "__8" <-{ PtrOp } CallE ptr_dangling_T_loc [] [@{expr} ];
+   Goto "_bb6"
+  ]>%E $
+  <[
+  "_bb0" :=
+   "__4" <-{ IntOp USize } CallE std_mem_size_of_T_loc [] [@{expr} ];
+   Goto "_bb4"
+  ]>%E $
+  <[
+  "_bb1" :=
+   "__2" <-{ BoolOp } val_of_bool true;
+   Goto "_bb3"
+  ]>%E $
+  <[
+  "_bb4" :=
+   "__3" <-{ BoolOp } (use{ IntOp USize } ("__4")) = { IntOp USize , IntOp USize , U8 } (I2v (0) U64);
+   if{ BoolOp }: use{ BoolOp } ("__3") then
+    Goto "_bb1"
+   else
+    Goto "_bb2"
+  ]>%E $
+  <[
+  "_bb3" :=
+   if{ BoolOp }: use{ BoolOp } ("__2") then
+    Goto "_bb5"
+   else
+    Goto "_bb7"
+  ]>%E $
+  ∅;
+ f_init := "_bb0";
+|}.
+
+Definition Vec_T_push_def (Vec_T_cap_T_loc : loc) (Vec_T_ptr_T_loc : loc) (ptr_add_T_loc : loc) (std_ptr_write_T_loc : loc) (RawVec_T_grow_T_loc : loc) (T_st : syn_type) : function := {|
+ f_args := [
+  ("self", void* : layout);
+  ("elem", (use_layout_alg' T_st) : layout)
+ ];
+ f_local_vars := [
+  ("__0", (layout_of unit_sl) : layout);
+  ("__3", (layout_of unit_sl) : layout);
+  ("__4", (it_layout U8) : layout);
+  ("__5", (it_layout USize) : layout);
+  ("__6", (it_layout USize) : layout);
+  ("__7", void* : layout);
+  ("__8", (layout_of unit_sl) : layout);
+  ("__9", void* : layout);
+  ("__10", (layout_of unit_sl) : layout);
+  ("__11", (layout_of unit_sl) : layout);
+  ("__12", void* : layout);
+  ("__13", void* : layout);
+  ("__14", void* : layout);
+  ("__15", (it_layout USize) : layout);
+  ("__16", (use_layout_alg' T_st) : layout);
+  ("__17", (it_layout USize) : layout)
+ ];
+ f_code :=
+  <[
+  "_bb6" :=
+   annot: EndLftAnnot "llft6";
+   "__15" <-{ IntOp USize } use{ IntOp USize } ((!{ PtrOp } ( "self" )) at{ ((Vec_sls (T_st))) } "len");
+   "__12" <-{ PtrOp } CallE ptr_add_T_loc [] [@{expr} use{ PtrOp } ("__13"); use{ IntOp USize } ("__15")];
+   Goto "_bb7"
+  ]>%E $
+  <[
+  "_bb0" :=
+   annot: CopyLftNameAnnot "plft7" "ulft__";
+   "__5" <-{ IntOp USize } use{ IntOp USize } ((!{ PtrOp } ( "self" )) at{ ((Vec_sls (T_st))) } "len");
+   annot: StartLftAnnot "llft4" ["plft7"];
+   "__7" <-{ PtrOp } AnnotExpr 0 (GetLftNamesAnnot (LftNameTreeRef "plft8" (LftNameTreeLeaf))) (&ref{ Shr, None, "llft4" } (!{ PtrOp } ( "self" )));
+   annot: CopyLftNameAnnot "plft11" "plft8";
+   "__6" <-{ IntOp USize } CallE Vec_T_cap_T_loc ["plft11"] [@{expr} use{ PtrOp } ("__7")];
+   annot: EndLftAnnot "llft4";
+   Goto "_bb1"
+  ]>%E $
+  <[
+  "_bb8" :=
+   "__10" <-{ StructOp unit_sl [] } zst_val;
+   "__17" <-{ IntOp USize } (use{ IntOp USize } ((!{ PtrOp } ( "self" )) at{ ((Vec_sls (T_st))) } "len")) +c{ IntOp USize , IntOp USize } (I2v (1) U64);
+   assert{ BoolOp }: (val_of_bool false) = { BoolOp , BoolOp , U8 } (val_of_bool false);
+   Goto "_bb9"
+  ]>%E $
+  <[
+  "_bb7" :=
+   "__16" <-{ (use_op_alg' T_st) } use{ (use_op_alg' T_st) } ("elem");
+   "__11" <-{ StructOp unit_sl [] } CallE std_ptr_write_T_loc [] [@{expr} AnnotExpr 1 ExtractValueAnnot (use{ PtrOp } ("__12")); use{ (use_op_alg' T_st) } ("__16")];
+   Goto "_bb8"
+  ]>%E $
+  <[
+  "_bb9" :=
+   (!{ PtrOp } ( "self" )) at{ ((Vec_sls (T_st))) } "len" <-{ IntOp USize } use{ IntOp USize } ("__17");
+   "__0" <-{ StructOp unit_sl [] } zst_val;
+   Goto "_bb10"
+  ]>%E $
+  <[
+  "_bb4" :=
+   "__3" <-{ StructOp unit_sl [] } zst_val;
+   Goto "_bb5"
+  ]>%E $
+  <[
+  "_bb1" :=
+   annot: EndLftAnnot "llft4";
+   "__4" <-{ BoolOp } (use{ IntOp USize } ("__5")) = { IntOp USize , IntOp USize , U8 } (use{ IntOp USize } ("__6"));
+   if{ BoolOp }: use{ BoolOp } ("__4") then
+    Goto "_bb2"
+   else
+    Goto "_bb4"
+  ]>%E $
+  <[
+  "_bb2" :=
+   annot: StartLftAnnot "llft5" ["plft7"];
+   "__9" <-{ PtrOp } AnnotExpr 0 (GetLftNamesAnnot (LftNameTreeRef "plft9" (LftNameTreeLeaf))) (&ref{ Mut, Some (RSTLitType ["RawVec_inv_t"] [RSTTyVar "T"]), "llft5" } ((!{ PtrOp } ( "self" )) at{ ((Vec_sls (T_st))) } "buf"));
+   annot: CopyLftNameAnnot "plft12" "plft9";
+   "__8" <-{ StructOp unit_sl [] } CallE RawVec_T_grow_T_loc ["plft12"] [@{expr} use{ PtrOp } ("__9")];
+   annot: EndLftAnnot "llft5";
+   Goto "_bb3"
+  ]>%E $
+  <[
+  "_bb3" :=
+   annot: EndLftAnnot "llft5";
+   "__3" <-{ StructOp unit_sl [] } zst_val;
+   Goto "_bb5"
+  ]>%E $
+  <[
+  "_bb10" :=
+   return (use{ StructOp unit_sl [] } ("__0"))
+  ]>%E $
+  <[
+  "_bb5" :=
+   annot: StartLftAnnot "llft6" ["plft7"];
+   "__14" <-{ PtrOp } AnnotExpr 0 (GetLftNamesAnnot (LftNameTreeRef "plft10" (LftNameTreeLeaf))) (&ref{ Shr, None, "llft6" } (!{ PtrOp } ( "self" )));
+   annot: CopyLftNameAnnot "plft13" "plft10";
+   "__13" <-{ PtrOp } CallE Vec_T_ptr_T_loc ["plft13"] [@{expr} use{ PtrOp } ("__14")];
+   annot: EndLftAnnot "llft6";
+   Goto "_bb6"
+  ]>%E $
+  ∅;
+ f_init := "_bb0";
+|}.
+
+Definition Vec_T_ptr_def (RawVec_T_ptr_T_loc : loc) (T_st : syn_type) : function := {|
+ f_args := [
+  ("self", void* : layout)
+ ];
+ f_local_vars := [
+  ("__0", void* : layout);
+  ("__2", void* : layout)
+ ];
+ f_code :=
+  <[
+  "_bb0" :=
+   annot: CopyLftNameAnnot "plft5" "ulft_a";
+   annot: CopyLftNameAnnot "plft4" "plft5";
+   "__2" <-{ PtrOp } AnnotExpr 0 (GetLftNamesAnnot (LftNameTreeRef "plft6" (LftNameTreeLeaf))) (&ref{ Shr, None, "plft4" } ((!{ PtrOp } ( "self" )) at{ ((Vec_sls (T_st))) } "buf"));
+   annot: CopyLftNameAnnot "plft7" "plft6";
+   "__0" <-{ PtrOp } CallE RawVec_T_ptr_T_loc ["plft7"] [@{expr} use{ PtrOp } ("__2")];
+   Goto "_bb1"
+  ]>%E $
+  <[
+  "_bb1" :=
+   (*annot: StratifyContextAnnot;*)
+   return (use{ PtrOp } ("__0"))
+  ]>%E $
+  ∅;
+ f_init := "_bb0";
+|}.
+
+Definition RawVec_T_grow_def (check_array_layoutable_T_loc : loc) (realloc_array_T_loc : loc) (alloc_array_T_loc : loc) (std_mem_size_of_T_loc : loc) (T_st : syn_type) : function := {|
+ f_args := [
+  ("self", void* : layout)
+ ];
+ f_local_vars := [
+  ("__0", (layout_of unit_sl) : layout);
+  ("__2", (layout_of unit_sl) : layout);
+  ("__3", (it_layout U8) : layout);
+  ("__4", (it_layout U8) : layout);
+  ("__5", (it_layout USize) : layout);
+  ("__6", (layout_of unit_sl) : layout);
+  ("new_cap", (it_layout USize) : layout);
+  ("__8", (it_layout U8) : layout);
+  ("__9", (it_layout USize) : layout);
+  ("__11", (it_layout USize) : layout);
+  ("__12", (it_layout USize) : layout);
+  ("__13", (layout_of unit_sl) : layout);
+  ("__14", (it_layout U8) : layout);
+  ("__15", (it_layout U8) : layout);
+  ("__16", (it_layout USize) : layout);
+  ("__17", (layout_of unit_sl) : layout);
+  ("new_ptr", void* : layout);
+  ("__19", (it_layout U8) : layout);
+  ("__20", (it_layout USize) : layout);
+  ("__21", (it_layout USize) : layout);
+  ("old_ptr", void* : layout);
+  ("__23", (it_layout USize) : layout);
+  ("__24", void* : layout);
+  ("__25", void* : layout);
+  ("__26", (it_layout USize) : layout);
+  ("__27", void* : layout);
+  ("__28", void* : layout);
+  ("__29", (it_layout USize) : layout)
+ ];
+ f_code :=
+  <[
+  "_bb1" :=
+   "__4" <-{ BoolOp } (use{ IntOp USize } ("__5")) != { IntOp USize , IntOp USize , U8 } (I2v (0) U64);
+   "__3" <-{ BoolOp } UnOp (NotBoolOp) (BoolOp) (use{ BoolOp } ("__4"));
+   if{ BoolOp }: use{ BoolOp } ("__3") then
+    Goto "_bb2"
+   else
+    Goto "_bb3"
+  ]>%E $
+  <[
+  "_bb8" :=
+   "__14" <-{ BoolOp } UnOp (NotBoolOp) (BoolOp) (use{ BoolOp } ("__15"));
+   if{ BoolOp }: use{ BoolOp } ("__14") then
+    Goto "_bb9"
+   else
+    Goto "_bb10"
+  ]>%E $
+  <[
+  "_bb10" :=
+   "__13" <-{ StructOp unit_sl [] } zst_val;
+   "__20" <-{ IntOp USize } use{ IntOp USize } ((!{ PtrOp } ( "self" )) at{ ((RawVec_sls (T_st))) } "cap");
+   "__19" <-{ BoolOp } (use{ IntOp USize } ("__20")) = { IntOp USize , IntOp USize , U8 } (I2v (0) U64);
+   if{ BoolOp }: use{ BoolOp } ("__19") then
+    Goto "_bb11"
+   else
+    Goto "_bb12"
+  ]>%E $
+  <[
+  "_bb6" :=
+   "new_cap" <-{ IntOp USize } use{ IntOp USize } ("__12");
+   "new_cap" <-{ IntOp USize } use{ IntOp USize } ("new_cap");
+   Goto "_bb7"
+  ]>%E $
+  <[
+  "_bb13" :=
+   Goto "_bb15"
+  ]>%E $
+  <[
+  "_bb3" :=
+   "__2" <-{ StructOp unit_sl [] } zst_val;
+   "__9" <-{ IntOp USize } use{ IntOp USize } ((!{ PtrOp } ( "self" )) at{ ((RawVec_sls (T_st))) } "cap");
+   "__8" <-{ BoolOp } (use{ IntOp USize } ("__9")) = { IntOp USize , IntOp USize , U8 } (I2v (0) U64);
+   if{ BoolOp }: use{ BoolOp } ("__8") then
+    Goto "_bb4"
+   else
+    Goto "_bb5"
+  ]>%E $
+  <[
+  "_bb11" :=
+   "__21" <-{ IntOp USize } use{ IntOp USize } ("new_cap");
+   "new_ptr" <-{ PtrOp } CallE alloc_array_T_loc [] [@{expr} use{ IntOp USize } ("__21")];
+   Goto "_bb13"
+  ]>%E $
+  <[
+  "_bb5" :=
+   "__11" <-{ IntOp USize } use{ IntOp USize } ((!{ PtrOp } ( "self" )) at{ ((RawVec_sls (T_st))) } "cap");
+   "__12" <-{ IntOp USize } (I2v (2) U64) ×c{ IntOp USize , IntOp USize } (use{ IntOp USize } ("__11"));
+   assert{ BoolOp }: (val_of_bool false) = { BoolOp , BoolOp , U8 } (val_of_bool false);
+   Goto "_bb6"
+  ]>%E $
+  <[
+  "_bb4" :=
+   "new_cap" <-{ IntOp USize } I2v (1) U64;
+   Goto "_bb7"
+  ]>%E $
+  <[
+  "_bb2" :=
+   StuckS
+  ]>%E $
+  <[
+  "_bb9" :=
+   StuckS
+  ]>%E $
+  <[
+  "_bb0" :=
+   annot: CopyLftNameAnnot "plft8" "ulft__";
+   "__5" <-{ IntOp USize } CallE std_mem_size_of_T_loc [] [@{expr} ];
+   Goto "_bb1"
+  ]>%E $
+  <[
+  "_bb15" :=
+   "__28" <-{ PtrOp } use{ PtrOp } ("new_ptr");
+   "__27" <-{ PtrOp } use{ PtrOp } ("__28");
+   (!{ PtrOp } ( "self" )) at{ ((RawVec_sls (T_st))) } "ptr" <-{ PtrOp } use{ PtrOp } ("__27");
+   "__29" <-{ IntOp USize } use{ IntOp USize } ("new_cap");
+   (!{ PtrOp } ( "self" )) at{ ((RawVec_sls (T_st))) } "cap" <-{ IntOp USize } use{ IntOp USize } ("__29");
+   "__0" <-{ StructOp unit_sl [] } zst_val;
+   (*annot: StratifyContextAnnot;*)
+   return (use{ StructOp unit_sl [] } ("__0"))
+  ]>%E $
+  <[
+  "_bb12" :=
+   "old_ptr" <-{ PtrOp } use{ PtrOp } ((!{ PtrOp } ( "self" )) at{ ((RawVec_sls (T_st))) } "ptr");
+   "__23" <-{ IntOp USize } use{ IntOp USize } ((!{ PtrOp } ( "self" )) at{ ((RawVec_sls (T_st))) } "cap");
+   "__25" <-{ PtrOp } use{ PtrOp } ("old_ptr");
+   "__24" <-{ PtrOp } use{ PtrOp } ("__25");
+   "__26" <-{ IntOp USize } use{ IntOp USize } ("new_cap");
+   "new_ptr" <-{ PtrOp } CallE realloc_array_T_loc [] [@{expr} use{ IntOp USize } ("__23"); AnnotExpr 1 ExtractValueAnnot (use{ PtrOp } ("__24")); use{ IntOp USize } ("__26")];
+   Goto "_bb14"
+  ]>%E $
+  <[
+  "_bb7" :=
+   "__16" <-{ IntOp USize } use{ IntOp USize } ("new_cap");
+   "__15" <-{ BoolOp } CallE check_array_layoutable_T_loc [] [@{expr} use{ IntOp USize } ("__16")];
+   Goto "_bb8"
+  ]>%E $
+  <[
+  "_bb14" :=
+   Goto "_bb15"
+  ]>%E $
+  ∅;
+ f_init := "_bb0";
+|}.
+
+Definition Vec_T_new_def (RawVec_T_new_T_loc : loc) (T_st : syn_type) : function := {|
+ f_args := [
+ ];
+ f_local_vars := [
+  ("__0", (use_layout_alg' (syn_type_of_sls ((Vec_sls (T_st))))) : layout);
+  ("__1", (use_layout_alg' (syn_type_of_sls ((RawVec_sls (T_st))))) : layout)
+ ];
+ f_code :=
+  <[
+  "_bb2" :=
+   (*annot: StratifyContextAnnot;*)
+   return (use{ (use_op_alg' (syn_type_of_sls ((Vec_sls (T_st))))) } ("__0"))
+  ]>%E $
+  <[
+  "_bb0" :=
+   "__1" <-{ (use_op_alg' (syn_type_of_sls ((RawVec_sls (T_st))))) } CallE RawVec_T_new_T_loc [] [@{expr} ];
+   Goto "_bb1"
+  ]>%E $
+  <[
+  "_bb1" :=
+   "__0" <-{ (use_op_alg' (syn_type_of_sls ((Vec_sls (T_st))))) } StructInit ((Vec_sls (T_st))) [("buf", use{ (use_op_alg' (syn_type_of_sls ((RawVec_sls (T_st))))) } ("__1") : expr); ("len", I2v (0) U64 : expr)];
+   (*expr: AnnotExpr 0 DropAnnot ("__1");*)
+   Goto "_bb2"
+  ]>%E $
+  ∅;
+ f_init := "_bb0";
+|}.
+
+Definition Vec_T_cap_def (T_st : syn_type) : function := {|
+ f_args := [
+  ("self", void* : layout)
+ ];
+ f_local_vars := [
+  ("__0", (it_layout USize) : layout)
+ ];
+ f_code :=
+  <[
+  "_bb0" :=
+   annot: CopyLftNameAnnot "plft4" "ulft_a";
+   "__0" <-{ IntOp USize } use{ IntOp USize } (((!{ PtrOp } ( "self" )) at{ ((Vec_sls (T_st))) } "buf") at{ ((RawVec_sls (T_st))) } "cap");
+   (*annot: StratifyContextAnnot;*)
+   return (use{ IntOp USize } ("__0"))
+  ]>%E $
+  ∅;
+ f_init := "_bb0";
+|}.
+
+Definition Vec_T_remove_def (std_ptr_copy_T_loc : loc) (Vec_T_ptr_T_loc : loc) (ptr_add_T_loc : loc) (std_ptr_read_T_loc : loc) (T_st : syn_type) : function := {|
+ f_args := [
+  ("self", void* : layout);
+  ("index", (it_layout USize) : layout)
+ ];
+ f_local_vars := [
+  ("__0", (use_layout_alg' T_st) : layout);
+  ("__3", (layout_of unit_sl) : layout);
+  ("__4", (it_layout U8) : layout);
+  ("__5", (it_layout U8) : layout);
+  ("__6", (it_layout USize) : layout);
+  ("__7", (it_layout USize) : layout);
+  ("__8", (layout_of unit_sl) : layout);
+  ("__9", (it_layout USize) : layout);
+  ("result", (use_layout_alg' T_st) : layout);
+  ("__11", void* : layout);
+  ("__12", void* : layout);
+  ("__13", void* : layout);
+  ("__14", void* : layout);
+  ("__15", (it_layout USize) : layout);
+  ("__16", (layout_of unit_sl) : layout);
+  ("__17", void* : layout);
+  ("__18", void* : layout);
+  ("__19", void* : layout);
+  ("__20", void* : layout);
+  ("__21", (it_layout USize) : layout);
+  ("__22", (it_layout USize) : layout);
+  ("__23", (it_layout USize) : layout);
+  ("__24", void* : layout);
+  ("__25", void* : layout);
+  ("__26", void* : layout);
+  ("__27", (it_layout USize) : layout);
+  ("__28", (it_layout USize) : layout);
+  ("__29", (it_layout USize) : layout);
+  ("__30", (it_layout USize) : layout);
+  ("__31", (it_layout USize) : layout)
+ ];
+ f_code :=
+  <[
+  "_bb8" :=
+   "__21" <-{ IntOp USize } use{ IntOp USize } ("__23");
+   "__18" <-{ PtrOp } CallE ptr_add_T_loc [] [@{expr} use{ PtrOp } ("__19"); use{ IntOp USize } ("__21")];
+   Goto "_bb9"
+  ]>%E $
+  <[
+  "_bb0" :=
+   annot: CopyLftNameAnnot "plft9" "ulft__";
+   "__6" <-{ IntOp USize } use{ IntOp USize } ("index");
+   "__7" <-{ IntOp USize } use{ IntOp USize } ((!{ PtrOp } ( "self" )) at{ ((Vec_sls (T_st))) } "len");
+   "__5" <-{ BoolOp } (use{ IntOp USize } ("__6")) <{ IntOp USize , IntOp USize , U8 } (use{ IntOp USize } ("__7"));
+   "__4" <-{ BoolOp } UnOp (NotBoolOp) (BoolOp) (use{ BoolOp } ("__5"));
+   if{ BoolOp }: use{ BoolOp } ("__4") then
+    Goto "_bb1"
+   else
+    Goto "_bb2"
+  ]>%E $
+  <[
+  "_bb3" :=
+   (!{ PtrOp } ( "self" )) at{ ((Vec_sls (T_st))) } "len" <-{ IntOp USize } use{ IntOp USize } ("__9");
+   annot: StartLftAnnot "llft6" ["plft9"];
+   "__14" <-{ PtrOp } AnnotExpr 0 (GetLftNamesAnnot (LftNameTreeRef "plft10" (LftNameTreeLeaf))) (&ref{ Shr, None, "llft6" } (!{ PtrOp } ( "self" )));
+   annot: CopyLftNameAnnot "plft13" "plft10";
+   "__13" <-{ PtrOp } CallE Vec_T_ptr_T_loc ["plft13"] [@{expr} use{ PtrOp } ("__14")];
+   annot: EndLftAnnot "llft6";
+   Goto "_bb4"
+  ]>%E $
+  <[
+  "_bb2" :=
+   "__3" <-{ StructOp unit_sl [] } zst_val;
+   "__9" <-{ IntOp USize } (use{ IntOp USize } ((!{ PtrOp } ( "self" )) at{ ((Vec_sls (T_st))) } "len")) -c{ IntOp USize , IntOp USize } (I2v (1) U64);
+   assert{ BoolOp }: (val_of_bool false) = { BoolOp , BoolOp , U8 } (val_of_bool false);
+   Goto "_bb3"
+  ]>%E $
+  <[
+  "_bb6" :=
+   annot: StartLftAnnot "llft7" ["plft9"];
+   "__20" <-{ PtrOp } AnnotExpr 0 (GetLftNamesAnnot (LftNameTreeRef "plft11" (LftNameTreeLeaf))) (&ref{ Shr, None, "llft7" } (!{ PtrOp } ( "self" )));
+   annot: CopyLftNameAnnot "plft14" "plft11";
+   "__19" <-{ PtrOp } CallE Vec_T_ptr_T_loc ["plft14"] [@{expr} use{ PtrOp } ("__20")];
+   annot: EndLftAnnot "llft7";
+   Goto "_bb7"
+  ]>%E $
+  <[
+  "_bb4" :=
+   annot: EndLftAnnot "llft6";
+   "__15" <-{ IntOp USize } use{ IntOp USize } ("index");
+   "__12" <-{ PtrOp } CallE ptr_add_T_loc [] [@{expr} use{ PtrOp } ("__13"); use{ IntOp USize } ("__15")];
+   Goto "_bb5"
+  ]>%E $
+  <[
+  "_bb7" :=
+   annot: EndLftAnnot "llft7";
+   "__22" <-{ IntOp USize } use{ IntOp USize } ("index");
+   "__23" <-{ IntOp USize } (use{ IntOp USize } ("__22")) +c{ IntOp USize , IntOp USize } (I2v (1) U64);
+   assert{ BoolOp }: (val_of_bool false) = { BoolOp , BoolOp , U8 } (val_of_bool false);
+   Goto "_bb8"
+  ]>%E $
+  <[
+  "_bb11" :=
+   "__29" <-{ IntOp USize } use{ IntOp USize } ((!{ PtrOp } ( "self" )) at{ ((Vec_sls (T_st))) } "len");
+   "__30" <-{ IntOp USize } use{ IntOp USize } ("index");
+   "__31" <-{ IntOp USize } (use{ IntOp USize } ("__29")) -c{ IntOp USize , IntOp USize } (use{ IntOp USize } ("__30"));
+   assert{ BoolOp }: (val_of_bool false) = { BoolOp , BoolOp , U8 } (val_of_bool false);
+   Goto "_bb12"
+  ]>%E $
+  <[
+  "_bb12" :=
+   "__28" <-{ IntOp USize } use{ IntOp USize } ("__31");
+   "__16" <-{ StructOp unit_sl [] } CallE std_ptr_copy_T_loc [] [@{expr} use{ PtrOp } ("__17"); use{ PtrOp } ("__24"); use{ IntOp USize } ("__28")];
+   Goto "_bb13"
+  ]>%E $
+  <[
+  "_bb9" :=
+   "__17" <-{ PtrOp } use{ PtrOp } ("__18");
+   annot: StartLftAnnot "llft8" ["plft9"];
+   "__26" <-{ PtrOp } AnnotExpr 0 (GetLftNamesAnnot (LftNameTreeRef "plft12" (LftNameTreeLeaf))) (&ref{ Shr, None, "llft8" } (!{ PtrOp } ( "self" )));
+   annot: CopyLftNameAnnot "plft15" "plft12";
+   "__25" <-{ PtrOp } CallE Vec_T_ptr_T_loc ["plft15"] [@{expr} use{ PtrOp } ("__26")];
+   annot: EndLftAnnot "llft8";
+   Goto "_bb10"
+  ]>%E $
+  <[
+  "_bb10" :=
+   annot: EndLftAnnot "llft8";
+   "__27" <-{ IntOp USize } use{ IntOp USize } ("index");
+   "__24" <-{ PtrOp } CallE ptr_add_T_loc [] [@{expr} use{ PtrOp } ("__25"); use{ IntOp USize } ("__27")];
+   Goto "_bb11"
+  ]>%E $
+  <[
+  "_bb1" :=
+   StuckS
+  ]>%E $
+  <[
+  "_bb13" :=
+   "__0" <-{ (use_op_alg' T_st) } use{ (use_op_alg' T_st) } ("result");
+   (*expr: AnnotExpr 0 DropAnnot ("result");*)
+   Goto "_bb14"
+  ]>%E $
+  <[
+  "_bb14" :=
+   (*annot: StratifyContextAnnot;*)
+   return (use{ (use_op_alg' T_st) } ("__0"))
+  ]>%E $
+  <[
+  "_bb5" :=
+   "__11" <-{ PtrOp } use{ PtrOp } ("__12");
+   "result" <-{ (use_op_alg' T_st) } CallE std_ptr_read_T_loc [] [@{expr} use{ PtrOp } ("__11")];
+   Goto "_bb6"
+  ]>%E $
+  ∅;
+ f_init := "_bb0";
+|}.
+
+Definition RawVec_T_ptr_def (T_st : syn_type) : function := {|
+ f_args := [
+  ("self", void* : layout)
+ ];
+ f_local_vars := [
+  ("__0", void* : layout);
+  ("__2", void* : layout)
+ ];
+ f_code :=
+  <[
+  "_bb0" :=
+   annot: CopyLftNameAnnot "plft4" "ulft__";
+   "__2" <-{ PtrOp } use{ PtrOp } ((!{ PtrOp } ( "self" )) at{ ((RawVec_sls (T_st))) } "ptr");
+   "__0" <-{ PtrOp } use{ PtrOp } ("__2");
+   (*annot: StratifyContextAnnot;*)
+   return (use{ PtrOp } ("__0"))
+  ]>%E $
+  ∅;
+ f_init := "_bb0";
+|}.
+
+Definition RawVec_T_cap_def (T_st : syn_type) : function := {|
+ f_args := [
+  ("self", void* : layout)
+ ];
+ f_local_vars := [
+  ("__0", (it_layout USize) : layout)
+ ];
+ f_code :=
+  <[
+  "_bb0" :=
+   annot: CopyLftNameAnnot "plft4" "ulft__";
+   "__0" <-{ IntOp USize } use{ IntOp USize } ((!{ PtrOp } ( "self" )) at{ ((RawVec_sls (T_st))) } "cap");
+   (*annot: StratifyContextAnnot;*)
+   return (use{ IntOp USize } ("__0"))
+  ]>%E $
+  ∅;
+ f_init := "_bb0";
+|}.
+
+Definition RawVec_T_new_def (ptr_dangling_T_loc : loc) (std_mem_size_of_T_loc : loc) (T_st : syn_type) : function := {|
+ f_args := [
+ ];
+ f_local_vars := [
+  ("__0", (use_layout_alg' (syn_type_of_sls ((RawVec_sls (T_st))))) : layout);
+  ("cap", (it_layout USize) : layout);
+  ("__2", (it_layout U8) : layout);
+  ("__3", (it_layout USize) : layout);
+  ("__4", void* : layout);
+  ("__5", void* : layout);
+  ("__6", (it_layout USize) : layout);
+  ("__7", (layout_of unit_sl) : layout)
+ ];
+ f_code :=
+  <[
+  "_bb0" :=
+   "__3" <-{ IntOp USize } CallE std_mem_size_of_T_loc [] [@{expr} ];
+   Goto "_bb1"
+  ]>%E $
+  <[
+  "_bb2" :=
+   "cap" <-{ IntOp USize } UnOp (NotIntOp) (IntOp USize) (I2v (0) U64);
+   Goto "_bb4"
+  ]>%E $
+  <[
+  "_bb4" :=
+   "__5" <-{ PtrOp } CallE ptr_dangling_T_loc [] [@{expr} ];
+   Goto "_bb5"
+  ]>%E $
+  <[
+  "_bb1" :=
+   "__2" <-{ BoolOp } (use{ IntOp USize } ("__3")) = { IntOp USize , IntOp USize , U8 } (I2v (0) U64);
+   if{ BoolOp }: use{ BoolOp } ("__2") then
+    Goto "_bb2"
+   else
+    Goto "_bb3"
+  ]>%E $
+  <[
+  "_bb5" :=
+   "__4" <-{ PtrOp } use{ PtrOp } ("__5");
+   "__6" <-{ IntOp USize } use{ IntOp USize } ("cap");
+   "__7" <-{ StructOp unit_sl [] } zst_val;
+   "__0" <-{ (use_op_alg' (syn_type_of_sls ((RawVec_sls (T_st))))) } StructInit ((RawVec_sls (T_st))) [("ptr", use{ PtrOp } ("__4") : expr); ("cap", use{ IntOp USize } ("__6") : expr); ("_marker", use{ StructOp unit_sl [] } ("__7") : expr)];
+   (*annot: StratifyContextAnnot;*)
+   return (use{ (use_op_alg' (syn_type_of_sls ((RawVec_sls (T_st))))) } ("__0"))
+  ]>%E $
+  <[
+  "_bb3" :=
+   "cap" <-{ IntOp USize } I2v (0) U64;
+   Goto "_bb4"
+  ]>%E $
+  ∅;
+ f_init := "_bb0";
+|}.
+
+Definition Vec_T_get_mut_def (Vec_T_get_unchecked_mut_T_loc : loc) (Vec_T_len_T_loc : loc) (T_st : syn_type) : function := {|
+ f_args := [
+  ("self", void* : layout);
+  ("index", (it_layout USize) : layout)
+ ];
+ f_local_vars := [
+  ("__0", (use_layout_alg' (syn_type_of_els ((std_option_Option_els (PtrSynType))))) : layout);
+  ("__3", (it_layout U8) : layout);
+  ("__4", (it_layout USize) : layout);
+  ("__5", (it_layout USize) : layout);
+  ("__6", void* : layout);
+  ("__7", void* : layout);
+  ("__8", void* : layout);
+  ("__9", void* : layout);
+  ("__10", (it_layout USize) : layout)
+ ];
+ f_code := 
+  <[
+  "_bb3" :=
+   annot: StartLftAnnot "llft6" ["plft14"];
+   "__7" <-{ PtrOp } AnnotExpr 0 (GetLftNamesAnnot (LftNameTreeRef "plft13" (LftNameTreeLeaf))) (&ref{ Mut, Some (RSTTyVar "T"), "llft6" } (!{ PtrOp } ( "__8" )));
+   (* TODO inserted the right lifetime manually *)
+   "__0" <-{ (use_op_alg' (syn_type_of_els ((std_option_Option_els (PtrSynType))))) } EnumInit ((std_option_Option_els (PtrSynType))) "Some" (RSTLitType ["std_option_Option_ty"] [RSTRef Mut "plft13" (RSTTyVar "T")]) (StructInit ((std_option_Option_Some_sls (PtrSynType))) [("0", use{ PtrOp } ("__7") : expr)]);
+   (* TODO manually inserted extendlft *)
+   annot: ExtendLftAnnot "llft5";
+   annot: ExtendLftAnnot "llft6";
+   Goto "_bb5"
+  ]>%E $
+  <[
+  "_bb4" :=
+  (* TODO inserted the right lifetime manually *)
+   "__0" <-{ (use_op_alg' (syn_type_of_els ((std_option_Option_els (PtrSynType))))) } EnumInit ((std_option_Option_els (PtrSynType))) "None" (RSTLitType ["std_option_Option_ty"] [RSTRef Mut "plft11" (RSTTyVar "T")]) (StructInit (std_option_Option_None_sls) []);
+   Goto "_bb5"
+  ]>%E $
+  <[
+  "_bb2" :=
+   annot: StartLftAnnot "llft5" ["plft11"];
+   "__9" <-{ PtrOp } AnnotExpr 0 (GetLftNamesAnnot (LftNameTreeRef "plft15" (LftNameTreeLeaf))) (&ref{ Mut, Some (RSTLitType ["Vec_inv_t"] [RSTTyVar "T"]), "llft5" } (!{ PtrOp } ( "self" )));
+   "__10" <-{ IntOp USize } use{ IntOp USize } ("index");
+   annot: CopyLftNameAnnot "plft17" "plft15";
+   "__8" <-{ PtrOp } CallE Vec_T_get_unchecked_mut_T_loc ["plft17"] [@{expr} use{ PtrOp } ("__9"); use{ IntOp USize } ("__10")];
+   (* TODO manually inserted *)
+   annot: CopyLftNameAnnot "plft14" "plft17";
+   Goto "_bb3"
+  ]>%E $
+  <[
+  "_bb0" :=
+   annot: CopyLftNameAnnot "plft11" "ulft__";
+   "__4" <-{ IntOp USize } use{ IntOp USize } ("index");
+   annot: StartLftAnnot "llft4" ["plft11"];
+   "__6" <-{ PtrOp } AnnotExpr 0 (GetLftNamesAnnot (LftNameTreeRef "plft12" (LftNameTreeLeaf))) (&ref{ Shr, None, "llft4" } (!{ PtrOp } ( "self" )));
+   annot: CopyLftNameAnnot "plft16" "plft12";
+   "__5" <-{ IntOp USize } CallE Vec_T_len_T_loc ["plft16"] [@{expr} use{ PtrOp } ("__6")];
+   annot: EndLftAnnot "llft4";
+   Goto "_bb1"
+  ]>%E $
+  <[
+  "_bb1" :=
+   annot: EndLftAnnot "llft4";
+   "__3" <-{ BoolOp } (use{ IntOp USize } ("__4")) <{ IntOp USize , IntOp USize , U8 } (use{ IntOp USize } ("__5"));
+   if{ BoolOp }: use{ BoolOp } ("__3") then
+    Goto "_bb2"
+   else
+    Goto "_bb4"
+  ]>%E $
+  <[
+  "_bb5" :=
+   return (use{ (use_op_alg' (syn_type_of_els ((std_option_Option_els (PtrSynType))))) } ("__0"))
+  ]>%E $
+  ∅;
+ f_init := "_bb0";
+|}.
+
+
+Definition Vec_T_get_def (Vec_T_len_T_loc : loc) (Vec_T_get_unchecked_T_loc : loc) (T_st : syn_type) : function := {|
+ f_args := [
+  ("self", void* : layout);
+  ("index", (it_layout USize) : layout)
+ ];
+ f_local_vars := [
+  ("__0", (use_layout_alg' (syn_type_of_els ((std_option_Option_els (PtrSynType))))) : layout);
+  ("__3", (it_layout U8) : layout);
+  ("__4", (it_layout USize) : layout);
+  ("__5", (it_layout USize) : layout);
+  ("__6", void* : layout);
+  ("__7", void* : layout);
+  ("__8", void* : layout);
+  ("__9", void* : layout);
+  ("__10", (it_layout USize) : layout)
+ ];
+ f_code := 
+  <[
+  "_bb1" :=
+   "__3" <-{ BoolOp } (use{ IntOp USize } ("__4")) <{ IntOp USize , IntOp USize , U8 } (use{ IntOp USize } ("__5"));
+   if{ BoolOp }: use{ BoolOp } ("__3") then
+    Goto "_bb2"
+   else
+    Goto "_bb4"
+  ]>%E $
+  <[
+  "_bb4" :=
+   (* TODO manually inserted the right lifetime *)
+   "__0" <-{ (use_op_alg' (syn_type_of_els ((std_option_Option_els (PtrSynType))))) } EnumInit ((std_option_Option_els (PtrSynType))) "None" (RSTLitType ["std_option_Option_ty"] [RSTRef Shr "plft16" (RSTTyVar "T")]) (StructInit (std_option_Option_None_sls) []);
+   Goto "_bb5"
+  ]>%E $
+  <[
+  "_bb0" :=
+   annot: CopyLftNameAnnot "plft11" "ulft__";
+   "__4" <-{ IntOp USize } use{ IntOp USize } ("index");
+   annot: CopyLftNameAnnot "plft4" "plft11";
+   "__6" <-{ PtrOp } AnnotExpr 0 (GetLftNamesAnnot (LftNameTreeRef "plft12" (LftNameTreeLeaf))) (&ref{ Shr, None, "plft4" } (!{ PtrOp } ( "self" )));
+   annot: CopyLftNameAnnot "plft16" "plft12";
+   "__5" <-{ IntOp USize } CallE Vec_T_len_T_loc ["plft16"] [@{expr} use{ PtrOp } ("__6")];
+   Goto "_bb1"
+  ]>%E $
+  <[
+  "_bb5" :=
+   return (use{ (use_op_alg' (syn_type_of_els ((std_option_Option_els (PtrSynType))))) } ("__0"))
+  ]>%E $
+  <[
+  "_bb2" :=
+   annot: CopyLftNameAnnot "plft5" "plft11";
+   "__9" <-{ PtrOp } AnnotExpr 0 (GetLftNamesAnnot (LftNameTreeRef "plft15" (LftNameTreeLeaf))) (&ref{ Shr, None, "plft5" } (!{ PtrOp } ( "self" )));
+   "__10" <-{ IntOp USize } use{ IntOp USize } ("index");
+   annot: CopyLftNameAnnot "plft17" "plft15";
+   "__8" <-{ PtrOp } CallE Vec_T_get_unchecked_T_loc ["plft17"] [@{expr} use{ PtrOp } ("__9"); use{ IntOp USize } ("__10")];
+   annot: CopyLftNameAnnot "plft14" "plft17";
+   Goto "_bb3"
+  ]>%E $
+  <[
+  "_bb3" :=
+   annot: CopyLftNameAnnot "plft6" "plft14";
+   "__7" <-{ PtrOp } AnnotExpr 0 (GetLftNamesAnnot (LftNameTreeRef "plft13" (LftNameTreeLeaf))) (&ref{ Shr, None, "plft6" } (!{ PtrOp } ( "__8" )));
+   (* TODO manually inserted the right lifetime *)
+   "__0" <-{ (use_op_alg' (syn_type_of_els ((std_option_Option_els (PtrSynType))))) } EnumInit ((std_option_Option_els (PtrSynType))) "Some" (RSTLitType ["std_option_Option_ty"] [RSTRef Shr "plft13" (RSTTyVar "T")]) (StructInit ((std_option_Option_Some_sls (PtrSynType))) [("0", use{ PtrOp } ("__7") : expr)]);
+   Goto "_bb5"
+  ]>%E $
+  ∅;
+ f_init := "_bb0";
+|}.
+
+
+
+Definition Vec_T_get_unchecked_mut_def (Vec_T_ptr_T_loc : loc) (ptr_add_T_loc : loc) (T_st : syn_type) : function := {|
+ f_args := [
+  ("self", void* : layout);
+  ("index", (it_layout USize) : layout)
+ ];
+ f_local_vars := [
+  ("__0", void* : layout);
+  ("__3", void* : layout);
+  ("__4", void* : layout);
+  ("p", void* : layout);
+  ("__6", void* : layout);
+  ("__7", void* : layout);
+  ("__8", (it_layout USize) : layout);
+  ("__9", (it_layout USize) : layout);
+  ("ret", void* : layout)
+ ];
+ f_code :=
+  <[
+  "_bb0" :=
+   annot: CopyLftNameAnnot "plft11" "ulft__";
+   "__9" <-{ IntOp USize } use{ IntOp USize } ((!{ PtrOp } ( "self" )) at{ ((Vec_sls (T_st))) } "len");
+   annot: StartLftAnnot "llft4" ["plft11"];
+   "__7" <-{ PtrOp } AnnotExpr 0 (GetLftNamesAnnot (LftNameTreeRef "plft14" (LftNameTreeLeaf))) (&ref{ Shr, None, "llft4" } (!{ PtrOp } ( "self" )));
+   annot: CopyLftNameAnnot "plft16" "plft14";
+   "__6" <-{ PtrOp } CallE Vec_T_ptr_T_loc ["plft16"] [@{expr} use{ PtrOp } ("__7")];
+   annot: EndLftAnnot "llft4";
+   Goto "_bb1"
+  ]>%E $
+  <[
+  "_bb1" :=
+   annot: EndLftAnnot "llft4";
+   "__8" <-{ IntOp USize } use{ IntOp USize } ("index");
+   "p" <-{ PtrOp } CallE ptr_add_T_loc [] [@{expr} use{ PtrOp } ("__6"); use{ IntOp USize } ("__8")];
+   Goto "_bb2"
+  ]>%E $
+  <[
+  "_bb2" :=
+   annot: StartLftAnnot "llft6" ["plft11"];
+   "ret" <-{ PtrOp } AnnotExpr 0 (GetLftNamesAnnot (LftNameTreeRef "plft15" (LftNameTreeLeaf))) (&ref{ Mut, Some (RSTTyVar "T"), "llft6" } (!{ PtrOp } ( "p" )));
+   annot: ExtendLftAnnot "llft6";
+   (* TODO I edited the code, some of the annotations currently are wrong *)
+   (*"ret" <-{ PtrOp } AnnotExpr 0 (GetLftNamesAnnot (LftNameTreeRef "plft15" (LftNameTreeLeaf))) (&ref{ Mut, Some (RSTTyVar "T"), "plft5" } (!{ PtrOp } ( "p" )));*)
+   (*annot: StartLftAnnot "llft6" ["plft15"];*)
+   (*"__4" <-{ PtrOp } AnnotExpr 0 (GetLftNamesAnnot (LftNameTreeRef "plft13" (LftNameTreeLeaf))) (&ref{ Mut, Some (RSTTyVar "T"), "llft6" } (!{ PtrOp } ( "ret" )));*)
+   (*annot: StartLftAnnot "llft7" ["plft13"];*)
+   (*"__3" <-{ PtrOp } AnnotExpr 0 (GetLftNamesAnnot (LftNameTreeRef "plft12" (LftNameTreeLeaf))) (&ref{ Mut, Some (RSTTyVar "T"), "llft7" } (!{ PtrOp } ( "__4" )));*)
+   (*annot: StartLftAnnot "llft8" ["plft12"];*)
+   (*"__0" <-{ PtrOp } AnnotExpr 0 (GetLftNamesAnnot (LftNameTreeRef "plft10" (LftNameTreeLeaf))) (&ref{ Mut, Some (RSTTyVar "T"), "llft8" } (!{ PtrOp } ( "__3" )));*)
+
+   (*annot: StratifyContextAnnot;*)
+   return (use{ PtrOp } ("ret"))
+  ]>%E $
+  ∅;
+ f_init := "_bb0";
+|}.
+
+Definition Vec_T_len_def (T_st : syn_type) : function := {|
+ f_args := [
+  ("self", void* : layout)
+ ];
+ f_local_vars := [
+  ("__0", (it_layout USize) : layout)
+ ];
+ f_code :=
+  <[
+  "_bb0" :=
+   annot: CopyLftNameAnnot "plft4" "ulft__";
+   "__0" <-{ IntOp USize } use{ IntOp USize } ((!{ PtrOp } ( "self" )) at{ ((Vec_sls (T_st))) } "len");
+   (*annot: StratifyContextAnnot;*)
+   return (use{ IntOp USize } ("__0"))
+  ]>%E $
+  ∅;
+ f_init := "_bb0";
+|}.
+
+Definition Vec_T_pop_def (Vec_T_ptr_T_loc : loc) (std_ptr_read_T_loc : loc) (ptr_add_T_loc : loc) (T_st : syn_type) : function := {|
+ f_args := [
+  ("self", void* : layout)
+ ];
+ f_local_vars := [
+  ("__0", (use_layout_alg' (syn_type_of_els ((std_option_Option_els (T_st))))) : layout);
+  ("__2", (it_layout U8) : layout);
+  ("__3", (it_layout USize) : layout);
+  ("__4", (it_layout USize) : layout);
+  ("__5", (use_layout_alg' T_st) : layout);
+  ("__6", void* : layout);
+  ("__7", void* : layout);
+  ("__8", void* : layout);
+  ("__9", void* : layout);
+  ("__10", (it_layout USize) : layout)
+ ];
+ f_code :=
+  <[
+  "_bb3" :=
+   (!{ PtrOp } ( "self" )) at{ ((Vec_sls (T_st))) } "len" <-{ IntOp USize } use{ IntOp USize } ("__4");
+   annot: StartLftAnnot "llft4" ["plft5"];
+   "__9" <-{ PtrOp } AnnotExpr 0 (GetLftNamesAnnot (LftNameTreeRef "plft6" (LftNameTreeLeaf))) (&ref{ Shr, None, "llft4" } (!{ PtrOp } ( "self" )));
+   annot: CopyLftNameAnnot "plft7" "plft6";
+   "__8" <-{ PtrOp } CallE Vec_T_ptr_T_loc ["plft7"] [@{expr} use{ PtrOp } ("__9")];
+   annot: EndLftAnnot "llft4";
+   Goto "_bb4"
+  ]>%E $
+  <[
+  "_bb6" :=
+   "__0" <-{ (use_op_alg' (syn_type_of_els ((std_option_Option_els (T_st))))) } EnumInit ((std_option_Option_els (T_st))) "Some" (RSTLitType ["std_option_Option_ty"] [RSTTyVar "T"]) (StructInit ((std_option_Option_Some_sls (T_st))) [("0", use{ (use_op_alg' T_st) } ("__5") : expr)]);
+   (*expr: AnnotExpr 0 DropAnnot ("__5");*)
+   Goto "_bb7"
+  ]>%E $
+  <[
+  "_bb0" :=
+   annot: CopyLftNameAnnot "plft5" "ulft__";
+   "__3" <-{ IntOp USize } use{ IntOp USize } ((!{ PtrOp } ( "self" )) at{ ((Vec_sls (T_st))) } "len");
+   "__2" <-{ BoolOp } (use{ IntOp USize } ("__3")) = { IntOp USize , IntOp USize , U8 } (I2v (0) U64);
+   if{ BoolOp }: use{ BoolOp } ("__2") then
+    Goto "_bb1"
+   else
+    Goto "_bb2"
+  ]>%E $
+  <[
+  "_bb4" :=
+   annot: EndLftAnnot "llft4";
+   "__10" <-{ IntOp USize } use{ IntOp USize } ((!{ PtrOp } ( "self" )) at{ ((Vec_sls (T_st))) } "len");
+   "__7" <-{ PtrOp } CallE ptr_add_T_loc [] [@{expr} use{ PtrOp } ("__8"); use{ IntOp USize } ("__10")];
+   Goto "_bb5"
+  ]>%E $
+  <[
+  "_bb7" :=
+   Goto "_bb8"
+  ]>%E $
+  <[
+  "_bb5" :=
+   "__6" <-{ PtrOp } use{ PtrOp } ("__7");
+   "__5" <-{ (use_op_alg' T_st) } CallE std_ptr_read_T_loc [] [@{expr} use{ PtrOp } ("__6")];
+   Goto "_bb6"
+  ]>%E $
+  <[
+  "_bb1" :=
+    (* TODO fixed the instantiation for the None variant here *)
+   "__0" <-{ (use_op_alg' (syn_type_of_els ((std_option_Option_els (T_st))))) } EnumInit ((std_option_Option_els (T_st))) "None" (RSTLitType ["std_option_Option_ty"] [RSTTyVar "T"]) (StructInit ((std_option_Option_None_sls )) []);
+   Goto "_bb8"
+  ]>%E $
+  <[
+  "_bb2" :=
+   "__4" <-{ IntOp USize } (use{ IntOp USize } ((!{ PtrOp } ( "self" )) at{ ((Vec_sls (T_st))) } "len")) -c{ IntOp USize , IntOp USize } (I2v (1) U64);
+   assert{ BoolOp }: (val_of_bool false) = { BoolOp , BoolOp , U8 } (val_of_bool false);
+   Goto "_bb3"
+  ]>%E $
+  <[
+  "_bb8" :=
+   return (use{ (use_op_alg' (syn_type_of_els ((std_option_Option_els (T_st))))) } ("__0"))
+  ]>%E $
+  ∅;
+ f_init := "_bb0";
+|}.
+
+(* TODO manually added Option::unwrap shim *)
+Definition std_option_Option_T_unwrap_def (T_st : syn_type) : function := {|
+ f_args := [
+  ("self", (use_layout_alg' (syn_type_of_els ((std_option_Option_els (T_st))))) : layout)
+ ];
+ f_local_vars := [
+  ("__0", (use_layout_alg' T_st) : layout);
+  ("__2", (it_layout ISize) : layout);
+  ("val", (use_layout_alg' T_st) : layout);
+  ("__4", (layout_of unit_sl) : layout)
+ ];
+ f_code := 
+  <[
+  "_bb6" :=
+   return (use{ (use_op_alg' T_st) } ("__0"))
+  ]>%E $
+  <[
+  "_bb3" :=
+   StuckS
+  ]>%E $
+  <[
+  "_bb4" :=
+   "val" <-{ (use_op_alg' T_st) } use{ (use_op_alg' T_st) } ((EnumData (((std_option_Option_els (T_st)))) "Some" ("self")) at{ ((std_option_Option_Some_sls (T_st))) } "0");
+   "__0" <-{ (use_op_alg' T_st) } use{ (use_op_alg' T_st) } ("val");
+   Goto "_bb5"
+  ]>%E $
+  <[
+  "_bb1" :=
+   StuckS
+  ]>%E $
+  <[
+  "_bb0" :=
+   "__2" <-{ IntOp ISize } use{ IntOp ISize } (EnumDiscriminant (((std_option_Option_els (T_st)))) ("self"));
+   Switch (ISize : int_type) (use{ IntOp ISize } ("__2")) (<[ 1%Z := 1%nat ]> $ <[ 0%Z := 0%nat ]> $ ∅) ([Goto "_bb1"; Goto "_bb2"]) (Goto "_bb3")
+  ]>%E $
+  <[
+  "_bb2" :=
+   Goto "_bb4"
+  ]>%E $
+  <[
+  "_bb5" :=
+   Goto "_bb6"
+  ]>%E $
+  ∅;
+ f_init := "_bb0";
+|}.
+
+
+Definition get_mut_client_def (Vec_T_new_i32_loc : loc) (Vec_T_push_i32_loc : loc) (Vec_T_get_mut_i32_loc : loc) (std_option_Option_unwrap_def_muti32_loc : loc) : function := {|
+ f_args := [
+ ];
+ f_local_vars := [
+  ("__0", (layout_of unit_sl) : layout);
+  ("x", (use_layout_alg' (syn_type_of_sls ((Vec_sls (IntSynType I32))))) : layout);
+  ("__2", (layout_of unit_sl) : layout);
+  ("__3", void* : layout);
+  ("__4", (layout_of unit_sl) : layout);
+  ("__5", void* : layout);
+  ("__6", (layout_of unit_sl) : layout);
+  ("__7", void* : layout);
+  ("xr", void* : layout);
+  ("__9", (use_layout_alg' (syn_type_of_els ((std_option_Option_els (PtrSynType))))) : layout);
+  ("__10", void* : layout);
+  ("__11", (layout_of unit_sl) : layout);
+  ("__12", (it_layout U8) : layout);
+  ("__13", (it_layout U8) : layout);
+  ("__14", (it_layout I32) : layout);
+  ("__15", (layout_of unit_sl) : layout);
+  ("__16", (layout_of unit_sl) : layout);
+  ("__17", (it_layout U8) : layout);
+  ("__18", (it_layout U8) : layout);
+  ("__19", (it_layout I32) : layout);
+  ("__20", void* : layout);
+  ("__21", (use_layout_alg' (syn_type_of_els ((std_option_Option_els (PtrSynType))))) : layout);
+  ("__22", void* : layout);
+  ("__23", (layout_of unit_sl) : layout)
+ ];
+ f_code := 
+  <[
+  "_bb9" :=
+   annot: CopyLftNameAnnot "plft10" "plft19";
+  (* TODO: currently this erroneously generates an instantiation for a lifetime ["plft10"]. Manually removed it. *)
+   "__20" <-{ PtrOp } CallE std_option_Option_unwrap_def_muti32_loc [] [@{expr} use{ (use_op_alg' (syn_type_of_els ((std_option_Option_els (PtrSynType))))) } ("__21")];
+   Goto "_bb10"
+  ]>%E $
+  <[
+  "_bb10" :=
+   "__19" <-{ IntOp I32 } use{ IntOp I32 } (!{ PtrOp } ( "__20" ));
+   "__18" <-{ BoolOp } (use{ IntOp I32 } ("__19")) = { IntOp I32 , IntOp I32 , U8 } (I2v (42) I32);
+   annot: EndLftAnnot "llft9";
+   "__17" <-{ BoolOp } UnOp (NotBoolOp) (BoolOp) (use{ BoolOp } ("__18"));
+   if{ BoolOp }: use{ BoolOp } ("__17") then
+    Goto "_bb11"
+   else
+    Goto "_bb12"
+  ]>%E $
+  <[
+  "_bb1" :=
+   annot: StartLftAnnot "llft3" [];
+   "__3" <-{ PtrOp } AnnotExpr 0 (GetLftNamesAnnot (LftNameTreeRef "plft12" (LftNameTreeLeaf))) (&ref{ Mut, Some (RSTLitType ["Vec_inv_t"] [RSTInt I32]), "llft3" } ("x"));
+   annot: CopyLftNameAnnot "plft21" "plft12";
+   "__2" <-{ StructOp unit_sl [] } CallE Vec_T_push_i32_loc ["plft21"] [@{expr} use{ PtrOp } ("__3"); I2v (100) I32];
+   annot: EndLftAnnot "llft3";
+   Goto "_bb2"
+  ]>%E $
+  <[
+  "_bb12" :=
+   "__16" <-{ StructOp unit_sl [] } zst_val;
+   "__0" <-{ StructOp unit_sl [] } zst_val;
+   (*expr: AnnotExpr 0 DropAnnot ("x");*)
+   Goto "_bb13"
+  ]>%E $
+  <[
+  "_bb13" :=
+   return (use{ StructOp unit_sl [] } ("__0"))
+  ]>%E $
+  <[
+  "_bb11" :=
+   StuckS
+  ]>%E $
+  <[
+  "_bb6" :=
+   "__14" <-{ IntOp I32 } use{ IntOp I32 } (!{ PtrOp } ( "xr" ));
+   "__13" <-{ BoolOp } (use{ IntOp I32 } ("__14")) = { IntOp I32 , IntOp I32 , U8 } (I2v (200) I32);
+   "__12" <-{ BoolOp } UnOp (NotBoolOp) (BoolOp) (use{ BoolOp } ("__13"));
+   if{ BoolOp }: use{ BoolOp } ("__12") then
+    Goto "_bb7"
+   else
+    Goto "_bb8"
+  ]>%E $
+  <[
+  "_bb4" :=
+   annot: EndLftAnnot "llft5";
+   annot: StartLftAnnot "llft6" [];
+   "__10" <-{ PtrOp } AnnotExpr 0 (GetLftNamesAnnot (LftNameTreeRef "plft17" (LftNameTreeLeaf))) (&ref{ Mut, Some (RSTLitType ["Vec_inv_t"] [RSTInt I32]), "llft6" } ("x"));
+   annot: CopyLftNameAnnot "plft24" "plft17";
+   "__9" <-{ (use_op_alg' (syn_type_of_els ((std_option_Option_els (PtrSynType))))) } CallE Vec_T_get_mut_i32_loc ["plft24"] [@{expr} use{ PtrOp } ("__10"); I2v (1) U64];
+   (* TODO fix update of lft name map here, manually added *)
+   annot: CopyLftNameAnnot "plft16" "plft24";
+   Goto "_bb5"
+  ]>%E $
+  <[
+  "_bb2" :=
+   annot: EndLftAnnot "llft3";
+   annot: StartLftAnnot "llft4" [];
+   "__5" <-{ PtrOp } AnnotExpr 0 (GetLftNamesAnnot (LftNameTreeRef "plft13" (LftNameTreeLeaf))) (&ref{ Mut, Some (RSTLitType ["Vec_inv_t"] [RSTInt I32]), "llft4" } ("x"));
+   annot: CopyLftNameAnnot "plft22" "plft13";
+   "__4" <-{ StructOp unit_sl [] } CallE Vec_T_push_i32_loc ["plft22"] [@{expr} use{ PtrOp } ("__5"); I2v (200) I32];
+   annot: EndLftAnnot "llft4";
+   Goto "_bb3"
+  ]>%E $
+  <[
+  "_bb5" :=
+   annot: CopyLftNameAnnot "plft7" "plft16";
+   (* TODO: currently this erroneously generates an instantiation for a lifetime ["plft7"]. Manually removed it. *)
+   "xr" <-{ PtrOp } CallE std_option_Option_unwrap_def_muti32_loc [] [@{expr} use{ (use_op_alg' (syn_type_of_els ((std_option_Option_els (PtrSynType))))) } ("__9")];
+   Goto "_bb6"
+  ]>%E $
+  <[
+  "_bb0" :=
+   "x" <-{ (use_op_alg' (syn_type_of_sls ((Vec_sls (IntSynType I32))))) } CallE Vec_T_new_i32_loc [] [@{expr} ];
+   Goto "_bb1"
+  ]>%E $
+  <[
+  "_bb8" :=
+   "__11" <-{ StructOp unit_sl [] } zst_val;
+   !{ PtrOp } ( "xr" ) <-{ IntOp I32 } I2v (42) I32;
+   annot: EndLftAnnot "llft6";
+   annot: StartLftAnnot "llft9" [];
+   "__22" <-{ PtrOp } AnnotExpr 0 (GetLftNamesAnnot (LftNameTreeRef "plft20" (LftNameTreeLeaf))) (&ref{ Mut, Some (RSTLitType ["Vec_inv_t"] [RSTInt I32]), "llft9" } ("x"));
+   annot: CopyLftNameAnnot "plft25" "plft20";
+   "__21" <-{ (use_op_alg' (syn_type_of_els ((std_option_Option_els (PtrSynType))))) } CallE Vec_T_get_mut_i32_loc ["plft25"] [@{expr} use{ PtrOp } ("__22"); I2v (1) U64];
+   (* TODO same *)
+   annot: CopyLftNameAnnot "plft19" "plft25";
+   Goto "_bb9"
+  ]>%E $
+  <[
+  "_bb7" :=
+   annot: EndLftAnnot "llft6";
+   StuckS
+  ]>%E $
+  <[
+  "_bb3" :=
+   annot: EndLftAnnot "llft4";
+   annot: StartLftAnnot "llft5" [];
+   "__7" <-{ PtrOp } AnnotExpr 0 (GetLftNamesAnnot (LftNameTreeRef "plft14" (LftNameTreeLeaf))) (&ref{ Mut, Some (RSTLitType ["Vec_inv_t"] [RSTInt I32]), "llft5" } ("x"));
+   annot: CopyLftNameAnnot "plft23" "plft14";
+   "__6" <-{ StructOp unit_sl [] } CallE Vec_T_push_i32_loc ["plft23"] [@{expr} use{ PtrOp } ("__7"); I2v (300) I32];
+   annot: EndLftAnnot "llft5";
+   Goto "_bb4"
+  ]>%E $
+  ∅;
+ f_init := "_bb0";
+|}.
+
+Definition Vec_T_get_unchecked_def (Vec_T_ptr_T_loc : loc) (ptr_add_T_loc : loc) (T_st : syn_type) : function := {|
+ f_args := [
+  ("self", void* : layout);
+  ("index", (it_layout USize) : layout)
+ ];
+ f_local_vars := [
+  ("__0", void* : layout);
+  ("__3", (it_layout USize) : layout);
+  ("p", void* : layout);
+  ("__5", void* : layout);
+  ("__6", void* : layout);
+  ("__7", (it_layout USize) : layout);
+  ("ret", void* : layout)
+ ];
+ f_code := 
+  <[
+  "_bb2" :=
+   (* TODO: manually constrained this by ulft__ *)
+   (* TODO maybe this should just be copylftannot instead? *)
+   annot: StartLftAnnot "plft5" ["ulft__"];
+   "ret" <-{ PtrOp } AnnotExpr 0 (GetLftNamesAnnot (LftNameTreeRef "plft11" (LftNameTreeLeaf))) (&ref{ Shr, None, "plft5" } (!{ PtrOp } ( "p" )));
+   annot: CopyLftNameAnnot "plft6" "plft11";
+   "__0" <-{ PtrOp } AnnotExpr 0 (GetLftNamesAnnot (LftNameTreeRef "plft8" (LftNameTreeLeaf))) (&ref{ Shr, None, "plft6" } (!{ PtrOp } ( "ret" )));
+   annot: ExtendLftAnnot "plft5";
+   return (use{ PtrOp } ("__0"))
+  ]>%E $
+  <[
+  "_bb1" :=
+   "__7" <-{ IntOp USize } use{ IntOp USize } ("index");
+   "p" <-{ PtrOp } CallE ptr_add_T_loc [] [@{expr} use{ PtrOp } ("__5"); use{ IntOp USize } ("__7")];
+   Goto "_bb2"
+  ]>%E $
+  <[
+  "_bb0" :=
+   annot: CopyLftNameAnnot "plft9" "ulft__";
+   "__3" <-{ IntOp USize } use{ IntOp USize } ((!{ PtrOp } ( "self" )) at{ ((Vec_sls (T_st))) } "len");
+   annot: CopyLftNameAnnot "plft4" "plft9";
+   "__6" <-{ PtrOp } AnnotExpr 0 (GetLftNamesAnnot (LftNameTreeRef "plft10" (LftNameTreeLeaf))) (&ref{ Shr, None, "plft4" } (!{ PtrOp } ( "self" )));
+   annot: CopyLftNameAnnot "plft12" "plft10";
+   "__5" <-{ PtrOp } CallE Vec_T_ptr_T_loc ["plft12"] [@{expr} use{ PtrOp } ("__6")];
+   Goto "_bb1"
+  ]>%E $
+  ∅;
+ f_init := "_bb0";
+|}.
+
+
+
+End code.
