rr_frontend/output/minivec_patched/generated_proof_Vec_T_get.v
@@ -1,0 +1,39 @@
+From caesium Require Import lang notation.
+From refinedrust Require Import typing shims.
+From refinedrust.examples.minivec_patched Require Import generated_code_minivec generated_specs_minivec extra_proofs_minivec.
+Set Default Proof Using "Type".
+
+Section proof.
+Context `{typeGS Σ}.
+
+Lemma Vec_T_get_proof (T_rt : Type) `{Inhabited T_rt} (T_st : syn_type) (Vec_T_len_T_loc : loc) (Vec_T_get_unchecked_T_loc : loc) (π : thread_id) :
+  syn_type_is_layoutable (T_st) →
+  syn_type_is_layoutable ((syn_type_of_sls ((Vec_sls (T_st))))) →
+  syn_type_is_layoutable ((syn_type_of_els ((std_option_Option_els (PtrSynType))))) →
+  Vec_T_len_T_loc ◁ᵥ{π} Vec_T_len_T_loc @ function_ptr [PtrSynType] (type_of_Vec_T_len (T_rt) (T_st)) -∗
+  Vec_T_get_unchecked_T_loc ◁ᵥ{π} Vec_T_get_unchecked_T_loc @ function_ptr [PtrSynType; IntSynType USize] (type_of_Vec_T_get_unchecked (T_rt) (T_st)) -∗
+  typed_function π (Vec_T_get_def Vec_T_len_T_loc Vec_T_get_unchecked_T_loc T_st) [(syn_type_of_els ((std_option_Option_els (PtrSynType)))); BoolSynType; IntSynType USize; IntSynType USize; PtrSynType; PtrSynType; PtrSynType; PtrSynType; IntSynType USize] (type_of_Vec_T_get T_rt T_st).
+Proof.
+  intros.
+  iStartProof.
+  start_function "Vec_T_get" ( [ [] ulft__] ) ( [ [  xs i ] T_ty ] ).
+  set (loop_map := BB_INV_MAP (PolyNil)).
+  intros arg_self arg_index local___0 local___3 local___4 local___5 local___6 local___7 local___8 local___9 local___10.
+  prepare_parameters ( xs i T_ty ).
+  init_lfts (named_lft_update "ulft__" ulft__ $ ∅ ).
+  init_tyvars ( <[ "T" := existT _ (T_ty) ]>%E $ ∅ ).
+
+  repeat liRStep; liShow.
+  all: rewrite /std_option_Option_ty.
+  all: repeat liRStep; liShow.
+  replace ((struct_t (std_option_Option_Some_sls PtrSynType) +[shr_ref T_ty ulft__])) with (std_option_Option_Some_ty (shr_ref T_ty ulft__)) by done.
+  repeat liRStep; liShow.
+
+  all: print_typesystem_goal "Vec_T_get".
+  Unshelve. 
+
+  all: unshelve_sidecond; sidecond_hook.
+  Unshelve. all: prepare_sideconditions; normalize_and_simpl_goal; try solve_goal; try (unfold_common_defs; solve_goal); unsolved_sidecond_hook.
+  Unshelve. all: try done; try apply: inhabitant; print_remaining_shelved_goal "Vec_T_get".
+Qed.
+End proof.
