rr_frontend/output/minivec_patched/generated_proof_Vec_T_len.v
@@ -1,0 +1,27 @@
+From caesium Require Import lang notation.
+From refinedrust Require Import typing.
+From refinedrust.examples.minivec_patched Require Import generated_code_minivec generated_specs_minivec.
+Set Default Proof Using "Type".
+
+Section proof.
+Context `{typeGS Σ}.
+Lemma Vec_T_len_proof (T_rt : Type) (T_st : syn_type)  (π : thread_id) :
+  syn_type_is_layoutable (T_st) →
+  syn_type_is_layoutable ((syn_type_of_sls ((Vec_sls (T_st))))) →
+  ⊢ typed_function π (Vec_T_len_def T_st) [IntSynType USize] (type_of_Vec_T_len T_rt T_st).
+Proof.
+  intros.
+  iStartProof.
+  start_function "Vec_T_len" ( [ [] ulft__] ) ( [  xs T_ty ] ).
+  set (loop_map := BB_INV_MAP (PolyNil)).
+  intros arg_self local___0.
+  prepare_parameters ( xs T_ty ).
+  init_lfts ( named_lft_update "ulft__" ulft__ $ ∅ ).
+  init_tyvars ( <[ "T" := existT _ (T_ty) ]>%E $ ∅ ).
+  repeat liRStep; liShow.
+  all: print_typesystem_goal "Vec_T_len".
+  Unshelve. all: unshelve_sidecond; sidecond_hook.
+  Unshelve. all: prepare_sideconditions; normalize_and_simpl_goal; try solve_goal; try (unfold_common_defs; solve_goal); unsolved_sidecond_hook.
+  Unshelve. all: try done; try apply: inhabitant; print_remaining_shelved_goal "Vec_T_len".
+Qed.
+End proof.
